a bunch of cleanup.

LogicalRelations.v
@@ -1,4 +1,3 @@
-
 Require Export Coq.Program.Tactics.
 Require Export Coq.Setoids.Setoid.
 Require Export Coq.Classes.Morphisms.
@@ -12,15 +11,30 @@ Require Export Coq.Relations.Relations.
 
 (* A distinguished equality for a given type is an equivalence marked as "the"
 equality for that type *)
-Polymorphic Class EqualsOp@{c} (A : Type@{c}) : Type :=
+ Class EqualsOp (A : Type) : Type :=
   equals : A -> A -> Prop.
 
 (* Distinguished equalities must be equivalences *)
-Polymorphic Class Equals@{c} (A : Type@{c}) `{EqOp:EqualsOp@{c} A} : Prop :=
+ Class Equals (A : Type) `{EqOp:EqualsOp A} : Prop :=
   { equals_equivalence :> Equivalence equals }.
 
-Notation "x '==' y" := (equals x y) (at level 80, no associativity).
+Global Instance Reflexive_equals `{Equals} : Reflexive equals.
+Proof.
+  apply equals_equivalence.
+Qed.
 
+
+Global Instance Symmetric_equals `{Equals} : Symmetric equals.
+Proof.
+  apply equals_equivalence.
+Qed.
+
+Global Instance Tansitive_equals `{Equals} : Transitive equals.
+Proof.
+  apply equals_equivalence.
+Qed.
+
+Notation "x '==' y" := (equals x y) (at level 80, no associativity).
 
 (***
  *** Equality Instances
@@ -29,28 +43,28 @@ Notation "x '==' y" := (equals x y) (at level 80, no associativity).
 (* Provable equality can be used as an instance of Equals, but we only give the
 definitions here, and do not declare them as instances, in case it is not *the*
 distinguished equality of a given type. *)
-Polymorphic Definition Eq_EqualsOp (A:Type) : EqualsOp A := eq.
-Polymorphic Definition Eq_Equals (A:Type) : Equals A (EqOp:=Eq_EqualsOp A).
+ Definition Eq_EqualsOp (A:Type) : EqualsOp A := eq.
+ Definition Eq_Equals (A:Type) : Equals A (EqOp:=Eq_EqualsOp A).
   repeat constructor; unfold equals, Eq_EqualsOp; auto with typeclass_instances.
 Qed.
 
 (* The equality on the unit type is the only thing it could be *)
-Polymorphic Instance Unit_EqualsOp : EqualsOp unit :=
+ Instance Unit_EqualsOp : EqualsOp unit :=
   fun p1 p2 => True.
 
 (* The unit equality is a valid equality *)
-Polymorphic Instance Unit_Equals : Equals unit.
+ Instance Unit_Equals : Equals unit.
   repeat constructor.
 Qed.
 
 
 (* Equality on pairs = equality on the two components *)
-Polymorphic Instance Pair_EqualsOp (A B: Type)
+ Instance Pair_EqualsOp (A B: Type)
             {EqOp_A:EqualsOp A} `{EqOp_B:EqualsOp B} : EqualsOp (A*B) :=
   fun p1 p2 => equals (fst p1) (fst p2) /\ equals (snd p1) (snd p2).
 
 (* Pair equality is a valid equality *)
-Polymorphic Instance Pair_Equals (A B: Type)
+ Instance Pair_Equals (A B: Type)
             `{Eq_A:Equals A} `{Eq_B:Equals B} : Equals (A*B).
   repeat constructor.
   reflexivity.
@@ -67,11 +81,11 @@ Qed.
  ***)
 
 (* A distinguished preorder is a preorder marked as "the" preorder for a type *)
-Polymorphic Class OrderOp@{c} (A : Type@{c}) : Type :=
+ Class OrderOp@{c} (A : Type@{c}) : Type :=
   order : A -> A -> Prop.
 
 (* Distinguished preorders must be preorders *)
-Polymorphic Class Order@{c} (A : Type@{c}) `{OrdOp:OrderOp@{c} A} : Prop :=
+ Class Order (A : Type) `{OrdOp:OrderOp A} : Prop :=
   { equals_preorder :> PreOrder order }.
 
 Notation "x '<~' y" := (order x y) (at level 80, no associativity).
@@ -84,9 +98,9 @@ Notation "x '<~' y" := (order x y) (at level 80, no associativity).
 (* If we have a distinguished preorder on a type, we want its distinguished
 equality to be the one that is induced by that preorder. Note: we give this a
 low priority, however, to favor other equality constructions. *)
-Polymorphic Instance Order_EqualsOp `{OrderOp} : EqualsOp A | 5 :=
+ Instance Order_EqualsOp `{OrderOp} : EqualsOp A | 5 :=
   fun x y => order x y /\ order y x.
-Polymorphic Instance Order_Equals `{Order} : Equals A | 5.
+ Instance Order_Equals `{Order} : Equals A | 5.
 repeat constructor.
 reflexivity.
 reflexivity.
@@ -98,8 +112,8 @@ Qed.
 
 (* Similarly, an equality can be used as a preorder, but we don't generally want
 this to be *the* preorder of a type *)
-Polymorphic Definition OrderOp_of_EqualsOp `{EqualsOp} : OrderOp A := equals.
-Polymorphic Definition Order_of_Equals `{Equals} : @Order A (OrderOp_of_EqualsOp).
+ Definition OrderOp_of_EqualsOp `{EqualsOp} : OrderOp A := equals.
+ Definition Order_of_Equals `{Equals} : @Order A (OrderOp_of_EqualsOp).
 repeat constructor; auto with typeclass_instances.
 Qed.
 
@@ -111,28 +125,28 @@ Qed.
 (* Provable equality can be used as an instance of Order, but we only give the
 definitions here, and do not declare them as instances, in case it is not *the*
 distinguished preorder of a given type. *)
-Polymorphic Definition Eq_OrderOp (A:Type) : OrderOp A := eq.
-Polymorphic Definition Eq_Order (A:Type) : Order A (OrdOp:=Eq_OrderOp A).
+ Definition Eq_OrderOp (A:Type) : OrderOp A := eq.
+ Definition Eq_Order (A:Type) : Order A (OrdOp:=Eq_OrderOp A).
   repeat constructor; unfold order, Eq_OrderOp; auto with typeclass_instances.
 Qed.
 
 (* The preorder on the unit type is the only thing it could be *)
-Polymorphic Instance Unit_OrderOp : OrderOp unit :=
+ Instance Unit_OrderOp : OrderOp unit :=
   fun p1 p2 => True.
 
 (* The unit preorder is a valid preorder *)
-Polymorphic Instance Unit_Order : Order unit.
+ Instance Unit_Order : Order unit.
   repeat constructor.
 Qed.
 
 
 (* The ordering on pairs = ordering on the two components *)
-Polymorphic Instance Pair_OrderOp (A B: Type)
+ Instance Pair_OrderOp (A B: Type)
             {OrdOp_A:OrderOp A} `{OrdOp_B:OrderOp B} : OrderOp (A*B) :=
   fun p1 p2 => order (fst p1) (fst p2) /\ order (snd p1) (snd p2).
 
 (* Pair equality is a valid equality *)
-Polymorphic Instance Pair_Order (A B: Type)
+ Instance Pair_Order (A B: Type)
             `{Ord_A:Order A} `{Ord_B:Order B} : Order (A*B).
   repeat constructor.
   reflexivity.
@@ -149,11 +163,11 @@ Qed.
 (* A logical relation is a relation between two types that respects the
 distinguished preorders of those two types; i.e., it is a morphism in the
 category of preorders. *)
-Polymorphic Class LogRelOp@{c} (A B : Type@{c}) : Type :=
+ Class LogRelOp@{c} (A B : Type@{c}) : Type :=
   relLR : A -> B -> Prop.
 
 (* The propositional part of a logical relation *)
-Polymorphic Class LogRel@{c} (A B : Type@{c})
+ Class LogRel@{c} (A B : Type@{c})
             `{OrdA:Order A} `{OrdB:Order B} `{LR:LogRelOp A B} : Prop :=
   { logrel_proper :> Proper (order ==> order ==> iff) (relLR (A:=A) (B:=B)) }.
 
@@ -163,7 +177,7 @@ Polymorphic Class LogRel@{c} (A B : Type@{c})
 (* equals respects itself *)
 (* FIXME: this is probably not needed...? *)
 (*
-Polymorphic Instance equals_proper `{LogRel} :
+ Instance equals_proper `{LogRel} :
   Proper (equals ==> equals ==> iff) equals.
 intros x1 x2 ex y1 y2 ey. rewrite ex.
  split; intro exy.
@@ -181,20 +195,20 @@ Qed.
 
 (* The identity logical relation, between a type and itself, is just the type's
 distinguished equality *)
-Polymorphic Instance LogRelOp_Id (A: Type) `{EqualsOp A} : LogRelOp A A :=
+ Instance LogRelOp_Id (A: Type) `{EqualsOp A} : LogRelOp A A :=
   equals.
 
-Polymorphic Instance LogRel_Id (A: Type) `{Equals A} : LogRel A A.
+ Instance LogRel_Id (A: Type) `{Equals A} : LogRel A A.
 constructor; intros x1 x2 ex y1 y2 ey.
 rewrite ex; rewrite ey; reflexivity.
 Qed.
 
 (* The logical relation for pairs: relate the components pointwise *)
-Polymorphic Instance LogRelOp_Pair (A1 A2 B1 B2: Type)
+ Instance LogRelOp_Pair (A1 A2 B1 B2: Type)
             `{LogRelOp A1 B1} `{LogRelOp A2 B2} : LogRelOp (A1*A2) (B1*B2) :=
   fun p1 p2 => fst p1 ~~ fst p2 /\ snd p1 ~~ snd p2.
 
-Polymorphic Instance LogRel_Pair (A1 A2 B1 B2: Type)
+~ Instance LogRel_Pair (A1 A2 B1 B2: Type)
             `{LogRel A1 B1} `{LogRel A2 B2} : LogRel (A1*A2) (B1*B2).
 constructor; intros p1 p1' e1 p2 p2' e2.
 destruct e1 as [e1_1 e1_2]; destruct e2 as [e2_1 e2_2].
