MonadState.v
@@ -1,37 +1,44 @@
+Require Import PredMonad.Monad.
 
-Add LoadPath "." as PredMonad.
-Require Export PredMonad.Monad.
+Global Instance EqualsOp_unit : EqualsOp unit :=
+{ equals := fun _ _ => True }.
+Instance Equals_unit : Equals unit.
+Proof.
+  constructor.
+  constructor; compute; tauto.
+Qed.
+
+Hint Extern 1 (EqualsOp unit) => exact EqualsOp_unit : typeclass_instances.
 
 
 (***
  *** Monads with State Effects
  ***)
 
-(* State effects = get and put *)
-Polymorphic Class MonadStateOps (S:Type) (M:Type -> Type) : Type :=
-  {
-    getM : M S;
-    putM : S -> M unit
+Section State.
+  Variables (S : Type) (M : Type -> Type).
+  (* State effects = get and put *)
+  Polymorphic Class MonadStateOps : Type :=
+  { getM : M S
+  ; putM : S -> M unit
   }.
+  Context `{Equals S} `{MonadOps M}.
 
-Polymorphic Class MonadState S `{Eq_S:Equals S} `{MonadOps}
-            `{MonadStateOps S M}
-            `{EqualsOp unit} (* FIXME: this should not be needed!  *)
-: Prop :=
+  Polymorphic Class MonadState (ms : MonadStateOps) : Prop :=
   {
     monad_state_monad :> Monad M;
     monad_state_get_get :
       forall A `{Eq_A:Equals A} f,
         bindM getM (fun s => bindM getM (f s)) ==
         (bindM getM (fun s => f s s) : M A);
-    monad_state_get_put : bindM getM putM == returnM tt;
+    monad_state_get_put : bindM getM putM == returnM tt ;
     monad_state_put_get :
       forall s, bindM (putM s) (fun _ => getM) ==
                 bindM (putM s) (fun _ => returnM s);
     monad_state_put_put :
       forall s1 s2, bindM (putM s1) (fun _ => putM s2) == putM s2
   }.
-
+End State.
 
 (***
  *** The State Monad Transformer
@@ -41,128 +48,116 @@ Section StateT.
 
 Context (S:Type).
 
+Record StateResult (T : Type) : Type := mkStResult
+{ state : S ; result : T }.
+
+Arguments mkStResult {_} _ _.
+Arguments state {_} _.
+Arguments result {_} _.
+
 (* NOTE: StateT requires that propositional equality, eq, be used as the
 distinguished equality for the state type, S. Otherwise, we need to restrict
 StateT to only contain Proper functions from S, which seems like a pain. *)
-Local Instance S_EqualsOp (S:Type) `{EqualsOp} : EqualsOp (prod S A) :=
-  Pair_EqualsOp S A (EqOp_A:=Eq_EqualsOp S).
-Local Instance S_Equals (S:Type) `{Equals} : Equals (prod S A) :=
-  Pair_Equals S A (Eq_A:=Eq_Equals S).
+Global Instance S_EqualsOp {A} `{EqualsOp A} : EqualsOp (StateResult A) :=
+  fun a b => a.(state) = b.(state) /\ equals a.(result) b.(result).
+Global Instance S_Equals {A} `{Equals A} : Equals (StateResult A).
+Proof.
+  constructor. constructor.
+  - constructor; auto. eapply reflexivity.
+  - red. destruct 1. constructor; auto. symmetry. auto.
+  - red. destruct 1. destruct 1. constructor. congruence. rewrite H1. assumption.
+Qed.
 
 (* StateT itself *)
-Definition StateT (M: Type -> Type) (X:Type) := S -> M (prod S X).
+Variable M : Type -> Type.
 
-Instance StateT_MonadOps `{MonadOps} : MonadOps (StateT M) :=
+Definition StateT (X:Type) := S -> M (StateResult X).
+
+Global Instance StateT_EqualsOp {A} `{MonadOps M} `{EqualsOp A} : EqualsOp (StateT A) :=
+  pointwise_relation S equals.
+Global Instance StateT_Equals {A} `{Monad M} `{Equals A} : Equals (StateT A).
+Proof.
+  constructor; constructor.
+  { red. intro. reflexivity. }
+  { red. intro. symmetry. assumption. }
+  { red. intro. etransitivity; eauto. }
+Qed.
+
+Global Instance StateT_MonadOps `{MonadOps M} : MonadOps StateT :=
   {returnM :=
-     fun A x => fun s => returnM (s, x);
+     fun A x => fun s => returnM (mkStResult s x);
    bindM :=
      fun A B m f =>
-       fun s => bindM (m s) (fun (sx:S * A) => let (s',x) := sx in f x s');
+       fun s => bindM (m s) (fun sx => let '(mkStResult s' x) := sx in f x s');
    equalsM :=
      fun {A} {EqualsOp} m1 m2 =>
-       forall s, equalsM (m1 s) (m2 s) }.
+       forall s, (m1 s) == (m2 s) }.
+
+Ltac tc := eauto with typeclass_instances.
 
 (* The Monad instance for StateT *)
-Instance StateT_Monad `{Monad} : Monad (StateT M).
+Global Instance StateT_Monad `{Monad M} : Monad (StateT).
   constructor; simpl; intros.
+  { red. intros.
+    rewrite (monad_return_bind (M:=M));
+      try auto with typeclass_instances; reflexivity. }
+  { red; intros.
+    etransitivity.
+    eapply (monad_proper_bind (M:=M)). tc. tc. reflexivity.
+    instantiate (1 := returnM).
+    red. intros. destruct x. eapply monad_proper_return; tc.
+    eapply (monad_bind_return (M:=M)). tc. }
+  { red. intros.
+    rewrite monad_assoc; tc.
+    eapply bind_fun_equalsM. intros.
+    destruct x. reflexivity. }
+  { eapply StateT_Equals. }
+  { red. red. intros.
+    eapply monad_proper_return; tc.
+    split. reflexivity. assumption. }
+  { do 4 red. intros.
+    eapply monad_proper_bind; tc.
+    red. intros.
+    destruct x1; destruct y1. destruct H4; simpl in *.
+    subst. eapply H3. assumption. }
+Qed.
 
-  intro; rewrite (monad_return_bind (M:=M));
-  try auto with typeclass_instances; reflexivity.
+Global Instance StateT_getM `{Monad M} : MonadStateOps S (StateT) :=
+{ getM := fun s => returnM (mkStResult s s)
+; putM := fun s_new s => returnM (mkStResult s_new tt) }.
 
-  intro; transitivity (bindM (m s) returnM);
-  [ | apply monad_bind_return; auto with typeclass_instances ].
-  eapply monad_proper_bind;
-    try auto with typeclass_instances; [ reflexivity | ].
-  intros p1 p2 ep; destruct p1; destruct p2.
-  apply monad_proper_return; [ auto with typeclass_instances | assumption ].
+Definition EqualsOp_Libniz (T : Type) : EqualsOp T := @eq T.
+Definition Equals_Libniz (T : Type) : @Equals T (EqualsOp_Libniz T).
+Proof.
+  constructor. compute. tc.
+Qed.
 
-  intro; rewrite monad_assoc; try auto with typeclass_instances.
-  apply bind_fun_equalsM; intro sx; destruct sx.
-  apply bind_fun_equalsM; intro sy; destruct sy.
-  reflexivity.
+Local Existing Instance Equals_Libniz.
 
-  constructor; constructor.
-  intros m s; reflexivity.
-  intros m1 m2 e s; symmetry; apply e.
-  intros m1 m2 m3 e1 e2 s; transitivity (m2 s); [ apply e1 | apply e2 ].
-
-  intros x y exy s;
-    apply monad_proper_return; [ auto with typeclass_instances | ].
-  split; [ reflexivity | assumption ].
-
-  intros m1 m2 em f1 f2 ef s.
-  eapply monad_proper_bind; try auto with typeclass_instances.
-  intros sx1 sx2 esx.
-  destruct sx1; destruct sx2; destruct esx as [esx1 esx2].
-  unfold fst in esx1; rewrite esx1.
-  eapply ef.
-  assumption.
+Instance StateT_MonadState `{Monad M}
+: @MonadState S StateT (EqualsOp_Libniz S) _ _.
+Proof.
+  constructor.
+  { eapply StateT_Monad. }
+  { intros.
+    do 3 red. intros.
+    unfold bindM. simpl.
+    repeat rewrite monad_return_bind; tc.
+    reflexivity. }
+  { do 3 red; intros. unfold bindM; simpl.
+    repeat rewrite monad_return_bind; tc.
+    reflexivity. }
+  { do 3 red. intros.
+    unfold bindM; simpl.
+    repeat rewrite monad_return_bind; tc. reflexivity. }
+  { do 3 red. intros.
+    unfold bindM; simpl.
+    repeat rewrite monad_return_bind; tc. reflexivity. }
 Qed.
 
 End StateT.
 
-
-FIXME HERE: update this MonadState instance
-
-(* The MonadState instance for StateT *)
-
-Instance StateT_getM {S} `{MonadRet} : MonadGet S (StateT S M) :=
-  fun s => returnM (s, s).
-Instance StateT_putM {S} `{MonadRet} : MonadPut S (StateT S M) :=
-  fun s_new s => returnM (s_new, tt).
-
-Instance StateT_MonadState S `{Monad} : MonadState S (StateT S M).
-  constructor; intros; try apply StateT_Monad;
-    unfold returnM, StateT_returnM, bindM, StateT_bindM,
-           getM, StateT_getM, putM, StateT_putM; intros;
-    try (intros; intro; repeat (rewrite monad_return_bind); reflexivity).
-  assumption.
-Qed.
+Arguments MonadState _ _ {_ _ _} : clear implicits.
 
 
-FIXME HERE: move all the following to a new file, MonadFix.v
 
-(***
- *** Non-Termination Effects
- ***)
-
-(* approxM m1 m2 means m1 "approximates" m2, i.e., m2 is "at least as
-terminating as" m1 *)
-Class MonadApprox (M:Type -> Type) : Type :=
-  approxM : forall {A}, relation (M A).
-
-Notation "m1 '<<<' m2" := (approxM m1 m2) (at level 80, no associativity).
-
-Class MonadFixM (M:Type -> Type) : Type :=
-  fixM : forall {A B}, ((A -> M B) -> (A -> M B)) -> A -> M B.
-
-Class MonadFix M {MonadRet:MonadRet M} {MonadBind:MonadBind M}
-      {MonadEquiv:MonadEquiv M} {MonadApprox:MonadApprox M}
-      {MonadFixM:MonadFixM M}
-: Prop :=
-  {
-    monad_fix_monad :> @Monad M MonadRet MonadBind MonadEquiv;
-    monad_fix_approx_preorder :> forall A, PreOrder (approxM (A:=A));
-    monad_fix_approx_antisymmetry :
-      forall A (m1 m2:M A), approxM m1 m2 -> approxM m2 m1 -> m1 == m2;
-    monad_fix_approx_bind :>
-      forall A B,
-        Proper
-          (approxM (A:=A) ==> (@eq A ==> approxM (A:=B)) ==> approxM (A:=B))
-          bindM;
-    monad_fix_approx_proper :>
-      forall A, Proper (eqM (A:=A) ==> eqM (A:=A) ==> iff) approxM;
-    monad_fix_fix_proper :>
-      forall A B,
-        Proper (((@eq A ==> eqM (A:=B)) ==> @eq A ==> eqM (A:=B))
-                  ==> @eq A ==> eqM (A:=B)) fixM;
-    monad_fix_fixm :
-      forall A B f x,
-        Proper (((@eq A) ==> (approxM (A:=B))) ==> @eq A ==> approxM (A:=B)) f ->
-        fixM (A:=A) (B:=B) f x == f (fixM f) x
-  }.
-
-Add Parametric Relation `{MonadFix} A : (M A) (approxM (A:=A))
-  reflexivity proved by PreOrder_Reflexive
-  transitivity proved by PreOrder_Transitive
-as approxM_morphism.
