MonadApprox.v
@@ -1,0 +1,45 @@
+Require Import PredMonad.Monad.
+(***
+ *** Non-Termination Effects
+ ***)
+
+Section Divergence.
+Variable M : Type -> Type.
+(* approxM m1 m2 means m1 "approximates" m2, i.e., m2 is "at least as
+terminating as" m1 *)
+Class MonadApprox : Type :=
+{ approxM : forall {A}, relation (M A)
+; fixM : forall {A B}, ((A -> M B) -> (A -> M B)) -> A -> M B }.
+
+Notation "m1 '<<<' m2" := (approxM m1 m2) (at level 80, no associativity).
+
+Class MonadFix `{Monad M} `{MonadApprox}
+: Prop :=
+  {
+    monad_fix_monad :> Monad M ;
+    monad_fix_approx_preorder :> forall A, PreOrder (approxM (A:=A));
+    monad_fix_approx_antisymmetry :
+      forall A (m1 m2:M A) `{Equals A}, approxM m1 m2 -> approxM m2 m1 -> m1 == m2;
+    monad_fix_approx_bind :>
+      forall A B `{Equals A} `{Equals B},
+        Proper
+          (approxM (A:=A) ==> (@eq A ==> approxM (A:=B)) ==> approxM (A:=B))
+          bindM ;
+    monad_fix_approx_proper :>
+      forall A `{Equals A}, Proper (equals (A:=M A) ==> equals (A:=M A) ==> iff) approxM;
+    monad_fix_fix_proper :>
+      forall A B `{Equals A} `{Equals B},
+        Proper (((@eq A ==> equals (A:=M B)) ==> @eq A ==> equals (A:=M B))
+                  ==> @eq A ==> equals (A:=M B)) fixM;
+    monad_fix_fixm :
+      forall A B f x `{Equals A} `{Equals B},
+        Proper (((@eq A) ==> (approxM (A:=B))) ==> @eq A ==> approxM (A:=B)) f ->
+        fixM (A:=A) (B:=B) f x == f (fixM f) x
+  }.
+
+Add Parametric Relation `{MonadFix} A : (M A) (approxM (A:=A))
+  reflexivity proved by PreOrder_Reflexive
+  transitivity proved by PreOrder_Transitive
+as approxM_morphism.
+
+End Divergence.
